Separate safe_to_remove

coq/def/Postcond.v
@@ -283,17 +283,17 @@ Module ForgetMemory.
     inv2.
 End ForgetMemory.
 
-Definition reduce_maydiff_non_physical (inv0: Invariant.t): Invariant.t :=
+(* Non-physical that is only in maydiff is safe to remove *)
+Definition safe_to_remove (inv0: Invariant.t) :=
   let used_ids := (Invariant.get_idTs_unary inv0.(Invariant.src))
-                    ++ (Invariant.get_idTs_unary inv0.(Invariant.tgt))
-  in
-  Invariant.update_maydiff
-    (IdTSet.filter
-       (fun idt => (Tag.eq_dec (fst idt) Tag.physical) ||
+                    ++ (Invariant.get_idTs_unary inv0.(Invariant.tgt)) in
+  (fun idt => (Tag.eq_dec (fst idt) Tag.physical) ||
                 if List.find (IdT.eq_dec idt) used_ids
                 then true
-                else false))
-    inv0.
+                else false).
+
+Definition reduce_maydiff_non_physical (inv0: Invariant.t): Invariant.t :=
+  Invariant.update_maydiff (IdTSet.filter (safe_to_remove inv0)) inv0.
 
 Definition reduce_maydiff_lessdef (inv0:Invariant.t): Invariant.t :=
   let lessdef_src := inv0.(Invariant.src).(Invariant.lessdef) in
